rupicola/README.md
@@ -43,8 +43,6 @@ The TODOs for the paper, are in the paper.
   - [ ] working on the running example (@Theo)
 
 - [ ] Admits
-  - [ ] Trace.fst
-    - [ ] 8 admits about traces and append
   - [ ] QTyp.fst 
     - [ ] `lem_substitution`
     ```fstar
@@ -58,14 +56,13 @@ The TODOs for the paper, are in the paper.
     - [ ] one case in `lem_shifting_preserves_closed`
     - [ ] admits and assumes in `lem_subst_freevars_closes_exp`
   - [ ] LogRelTargetSource.fst
-    - [ ] `safety_prod` (do we even need this?)
+    - [ ] `safety_prod` (we do not use this, do we need it?)
   - [ ] LogRelSourceTarget.CompatibilityLemmas.fst
     - [ ] 2 lemmas with silly assumes
   - [ ] LogRelTargetSource.CompatibilityLemmas.fst
     - [ ] 26 admitted compatibility lemmas
   - [ ] Compilation.fst
     - [ ] Two big assumes in `lem_compile_closed_valid`
-
 
 - [ ] Prepare artifact
   - [ ] Use the names from the paper in the artifact (e.g., rename STLC to LambdaIO)
